# Project 1 Assignment

Your first project will require you to answer each of the 10 questions below.  You will be expected to open a pull request with your initial answers by the second class meeting, giving you one week to work on these problems. You and your peers will then have one week to work together to refine your respective initial answers, so they are ready for final submission. Once your pull requests have been reviewed and merged to the development branch, I will review them, then merge to the master branch. 

Tip #1: Carefully study the Hedman selections assigned, as several of the questions are taken directly from the textbook. 
Tip #2: Google is your friend. An important skill to pick up in this class is recognizing when to think hard and when to think smart. You might find answers to some of the questions below simply by googling; you might find pieces of answers to parts of some question below, which will need to be combined; then again, you might not find any help at all because the questions are more novel than they initially appear. I encourage you to use existing resources as guidance, but be careful. My reputation for asking students tricky questions is well-earned. 
Tip #3: Work _together_ to solve these problems, even for initial submissions and when you do, document this in github. For example, you might feel like you nearly have answers to question 1, but would love another pair of eyes. You can then open a post in your local github account, and tag folks from class requesting they check out your work. 
Tip #4: The work we do is challenging; that should be assumed. You are smart enough to be here; that should also be assumed. We have neither time nor space for shaming, but all of time and space for praising. Be cognizant of how your messages might be received, and err on the side of caution. It is hard to surmise intent from text alone. For my part, I treat text only communications the way modern musicals are written: Little subtext; emotions on the sleeve. 
```

Note: The standard interpretation of the logical symbols - "∨", "∧", "→", "¬", "∀", "∃" - is assumed throughout. 

1. Provide the truth tables for each of the following propositional logic formulas. State whether each is a tautology, a contradiction, or contingent:
  ```
  (a) (¬A→B)∨((A∧¬C)→B) 
  

  A | B | C | (a)
|---|---|---|---|
  T | T | F | T
  T | T | F | T
  T | F | T | T
  F | T | T | T
  T | F | F | T
  F | T | F | T
  F | F | T | T
  F | F | F | T
  
  Tautology

  (b) (A→B)∧(A→¬B) 

  A | B| (b)
|---|---|---|
  T | T | F
  T | F | F
  F | T | T
  F | F | T

  Contingent

  (c) (A→(B∨C))∨(C→¬A) 

  A | B | C | (c)
|---|---|---|---|
  T | T | F | T 
  T | T | F | T 
  T | F | T | T
  F | T | T | T 
  T | F | F | T 
  F | T | F | T 
  F | F | T | T 
  F | F | F | T

  Tautology

  (d) ((A→B)∧C)∨(A∧D) 

  A | B | C | D | (d)
|---|---|---|---|---|
  T | T | T | T | T
  T | T | T | F | T
  T | T | F | T | T
  T | T | F | F | F
  T | F | T | T | T
  T | F | T | F | F
  T | F | F | T | T
  T | F | F | F | F
  F | T | T | T | T
  F | T | T | F | T
  F | T | F | T | F
  F | T | F | F | F
  F | F | T | T | T
  F | F | T | F | T
  F | F | F | T | F
  F | F | F | F | F

  Contingent
  ```
	
2. A _literal_ is an atomic formula or the negation of an atomic formula. We say a formula is in _conjunctive normal form_ (CNF) if it is the conjunction of the disjunction of literals. Find propositional logic formulas in CNF equivalent to each of the following:
  ```
  (a) (A→B)→C
  (¬A∨B)→C
  ¬(¬A∨B)∨C
  (A∧¬B)∨C
  (A∨C)∧(¬B∨C)  
  
  (b) (A→(B∨C))∨(C→¬A)
  It is a tautology. A∨¬A
  
The related truth table shows this formula is a tautology. The calculator gives me the same result. Giacomo and Karl wrote it is a tautology. However, I was not able to transform it into a CNF using Morgan's rules. Should I check at first the truth table and if it is a tautology then directly state that?

  (c) (¬A∧¬B∧C)∨(¬A∧¬C)∨(B∧C)∨A 
 It is a tautology. A∨¬A
  
The related truth table shows this formula is a tautology. The calculator gives me the same result. Giacomo and Karl wrote it is a tautology. However, I was not able to transform it into a CNF using Morgan's rules. Should I check at first the truth table and if it is a tautology then directly state that? Isn't a parenthesis missed in the first part (¬A∧¬B∧C)? Is it a formula then?

  I solved this question, using the Morgan's rules and checking Giacomo and Karl's answers.
  I also used this logic calculator: https://www.erpelstolz.at/gateway/formular-uk-zentral.html
```

3. Let V be the vocabulary of first-order logic consisting of a binary relation P and a unary relation F. Interpret P(x,y) as “x is a parent of y” and F(x) as “x is female.” Where possible define the following formulas in this vocabulary; where not possible, explain why: 
  
  ```
  (a)  B(x,y) that says that x is a brother of y  
  (b)  A(x,y) that says that x is an aunt of y  
  (c)  C(x,y) that says that x and y are cousins   
  (d)  O(x) that says that x is an only child  
  (e)  T(x) that says that x has exactly two brothers 
  
(a) B(x,y) that says that x is a brother of y
B(x,y) := ¬F(x)∧∃z(P(z,x)∧P(z,y)∧¬(x=y)∧¬(x=z))

Explanation: x is a brother of y if x is not female (¬F(x)) and there exists some z such that z is a parent of both x and y (P(z,x)∧P(z,y)), and x is not the same person as y (¬(x=y)), and x is not z (¬(x=z)). 

(b) A(x,y) that says that x is an aunt of y
A(x,y) := F(x)∧∃z(P(z,y)∧∃w(P(w,z)∧P(w,x))∧¬(x=w)))

Explanation: x is an aunt of y if x is female (F(x)) and there exists some z such that z is a parent of y (P(z,y)) and there exists some w such that w is a parent of both z and x (P(w,z)∧P(w,x)).

(c) C(x,y) that says that x and y are cousins
C(x,y) := ∃z∃w((¬(z=w)∧P(z,x))∧(P(w,y))∧∃u((P(u,z)∧P(u,w))∧¬(x=u)))

Explanation: x and y are cousins if there exist z and w such that z is not the same person as w (¬(z=w)), z is a parent of x (P(z,x)), w is a parent of y (P(w,y)), and there exists some u such that u is a parent of both z and w (P(u,z)∧P(u,w)).

(d) O(x) that says that x is an only child
O(x) := ∀y(P(y,x)→∀z(P(y,z)→(z=x)))

Explanation: x is an only child if for all y such that y is a parent of x (P(y,x)), for all z, if y is a parent of z then z must be x (P(y,z)→(z=x)).

(e) T(x) that says that x has exactly two brothers
T(x) := ∃y∃z(B(y,x)∧B(z,x))∧∀w(B(w,x)→((w=y)v(w=z)∧¬(x=y)∧¬(x=z)∧¬(z=y))))

Explanation: x has exactly two brothers if there exist y and z such that y is not the same person as z (¬(y=z)), both y and z are brothers of x (B(y,x)∧B(z,x)), and for all w, if w is a brother of x then w must be either y or z (B(w,x)→((w=y)∨(w=z))).

I worked on this question together with the other participants of the "Ontology Sprint" Workshop. We asked to answer this question to ChatGTP. Then, we work together on the generated solution. 
```

4. Let V be a vocabulary of the attribute (concept) language with complements (ALC) consisting of a role name "parent_of" and a concept name "Male". Interpret parent_of as "x is a parent of y" and M as "x is male". Where possible define the following formulas in this vocabulary; where not possible, explain why: 
```
  (a)  B that says that x is a brother of y
  (b)  A that says that x is an aunt of y
  (c)  C that says that x and y are cousins
  (d)  O that says that x is an only child  
  (e)  T that says that x has exactly two brothers 

From this point, Jisoo and I stated to work together.

(a)  B that says that x is a brother of y

This formula is impossible to define in ALC without ALCQ. We used ALCQ to define the formula. This is the best expression we got but we are not sure whether we can express that at least on child is male and the others can either be male or female. 

Person ≡ M ⊔ ¬M. p2 (parent of at least 2 children) ≡ ≥2 ∃parent_of.Person. 
B ≡ M ⊓ ≥2∃parent_of.Person

For now we stopped there as we wanted to move to the project 2. The project 2 first question has the same structure of this one. 
```

5. Select two formulas defined in ALC from question 4 to form the basis of a T-Box. Supplement this T-box with whatever other axioms you like, as well as an A-box, so that you ultimately construct a knowledge base K = (T,A). Provide a _model_ of K. This may be graphical or symbolic or both. 

We did not adress this question as we moved to the project 2. The project 2 second question has the same structure of this one.

6. Explain the difference - using natural language - between the first-order prefixes:
```
  (a) ∃x∀y and ∀x∃y
  (b) ∃x∀y∃z and ∀x∃y∀z 
  (c) ∀x∃y∀z∃w and ∃x∀y∃z∀w


(a) ∃x∀y and ∀x∃y
  The formula ∃x∀y means there is some x such that for all ys. Instead, ∀x∃y means for all xs there is  some y such that. 

(b) ∃x∀y∃z and ∀x∃y∀z 
  The formula  ∃x∀y∃z means there is some x such that for all ys there is some z. Instead, ∀x∃y∀z for all xs there is some y such that for all z.

(c) ∀x∃y∀z∃w and ∃x∀y∃z∀w
  The formula ∀x∃y∀z∃w means for all xs there is some y such that for all zs there is some w such that. Instead, the formula ∃x∀y∃z∀w means there is some x for all ys such as that there is some z for all ws.

We developped our answers comparing them to those of Giancomo and Karl and those found online.

The following answers ones have generated with help of ChatGPT.

a) ∃x∀y and ∀x∃y
"∃x∀y" asserts the existence of at least one element, denoted as "x," for which a particular condition holds for all possible elements denoted as "y."
"∀x∃y" asserts that, for every possible element x, there is at least one corresponding element y that satisfies a particular condition.

(b) ∃x∀y∃z and ∀x∃y∀z
"∃x∀y∃z" asserts the existence of at least one element, denoted as "x," for which a particular condition holds for all possible elements denoted as "y." And for each of these y, there exists at least one element "z" that satisfies a certain condition.
"∀x∃y∀z" asserts that for every possible element x, there exists at least one corresponding element y such that, for all possible elements z, a particular condition holds.

(c) ∀x∃y∀z∃w and ∃x∀y∃z∀w
"∀x∃y∀z∃w" asserts that for every possible element x, there exists at least one corresponding element y such that, for all possible elements z, there exists at least one w that satisfies a certain condition.
"∃x∀y∃z∀w" asserts the existence of at least one element x such that, for all possible elements y, there exists at least one z for which, for all possible elements w, a particular condition holds.
```

7. Show that the following sentences are not equivalent by exhibiting a graph that models one but not both of these sentences:
```
∀x∃y∀z(R(x,y) ∧ R(x,z) ∧ R(y,z))
∃x∀y∃z(R(x,y) ∧ R(x,z) ∧ R(y,z))


∀x∃y∀z(R(x,y) ∧ R(x,z) ∧ R(y,z))
   x
  / \
 y---z

∃x∀y∃z(R(x,y) ∧ R(x,z) ∧ R(y,z))
   x
   |
   |
  / \
 y   z
This was a tentative answer. To discuss more and improve.
```
	
8. Using an online tableau proof generator - such as the one found here `https://www.umsu.de/trees/` - provide tree proofs of the following entailments, which are known as the De Morgan's laws:
```
  (a) ∀x∀y(¬(Px ∧ Qx) → (¬Px ∨ ¬Qx))
  (b) ∀x∀y(¬(Px ∨ Qx) → (¬Px ∧ ¬Qx))
  (c) ∀x∀y((¬Px ∨ ¬Qx) → ¬(Px ∧ Qx))
  (d) ∀x∀y((¬Px ∧ ¬Qx) → ¬(Px ∨ Qx))

(a) ∀x∀y(¬(Px ∧ Qx) → (¬Px ∨ ¬Qx))

![proof](https://github.com/JisooSeo/PHI-696/assets/143667668/fe20e887-0569-4922-9bc5-994481aba1e5)

(b) ∀x∀y(¬(Px ∨ Qx) → (¬Px ∧ ¬Qx))

![proof (1)](https://github.com/JisooSeo/PHI-696/assets/143667668/5b4961c2-1179-4111-8a63-2098bd03649b)

(c) ∀x∀y((¬Px ∨ ¬Qx) → ¬(Px ∧ Qx))

![proof (2)](https://github.com/JisooSeo/PHI-696/assets/143667668/dc75d718-6d4a-4f31-9e83-cc949c1610c4)

(d) ∀x∀y((¬Px ∧ ¬Qx) → ¬(Px ∨ Qx))

![proof (3)](https://github.com/JisooSeo/PHI-696/assets/143667668/aa0cc56b-fd69-4564-8509-295a2b43ab03)
```

9. Using a natural deduction proof generator - such as the one found here `https://proofs.openlogicproject.org/` - provide natural deduction proofs for each of De Morgan's laws. 

```
(a) ∀x∀y(¬(Px ∧ Qx) → (¬Px ∨ ¬Qx))

∀x∀y(¬(Px ∧ Qx) → (¬Px ∨ ¬Qx)) [Given]
Let a be an arbitrary element. [Assumption for universal introduction]
Let b be an arbitrary element. [Assumption for universal introduction]
¬(Pa ∧ Qa) → (¬Pa ∨ ¬Qa) [Universal instantiation using a and b]
¬(Pa ∧ Qa) [Assumption for ¬-elimination]
¬Pa ∨ ¬Qa [Modus Ponens (4, 5)]
¬Qa ∨ ¬Pa [Commutation (6)]
¬Qa [Assumption for ∨-elimination]
¬Qa ∨ ¬Pa [Repetition (7)]
¬Pa [Disjunctive syllogism (8, 9)]
¬Pa ∨ ¬Qa [Repetition (10)]
(¬Pa ∨ ¬Qa) [∨-elimination (8-11)]
¬(Pa ∧ Qa) → (¬Pa ∨ ¬Qa) [→-introduction (5-12)]
∀y(¬(Pa ∧ Qa) → (¬Pa ∨ ¬Qa)) [∀-introduction (3-13)]
∀x∀y(¬(Px ∧ Qx) → (¬Px ∨ ¬Qx)) [∀-introduction (2-14)]

(b) ∀x∀y(¬(Px ∨ Qx) → (¬Px ∧ ¬Qx))

∀x∀y(¬(Px ∨ Qx) → (¬Px ∧ ¬Qx)) [Given]
Let a be an arbitrary element. [Assumption for universal introduction]
Let b be an arbitrary element. [Assumption for universal introduction]
¬(Pa ∨ Qa) → (¬Pa ∧ ¬Qa) [Universal instantiation using a and b]
¬(Pa ∨ Qa) [Assumption for →-elimination]
¬Pa ∧ ¬Qa [Modus Ponens (4, 5)]
¬Pa [Conjunction elimination (6)]
¬Qa [Conjunction elimination (6)]
¬Pa [∧-elimination (7)]
¬Qa [∧-elimination (8)]
¬Pa ∧ ¬Qa [∧-introduction (9, 10)]
(¬Pa ∧ ¬Qa) [→-introduction (5, 11)]
¬(Pa ∨ Qa) → (¬Pa ∧ ¬Qa) [→-introduction (5-12)]
∀y(¬(Pa ∨ Qa) → (¬Pa ∧ ¬Qa)) [∀-introduction (3-13)]
∀x∀y(¬(Px ∨ Qx) → (¬Px ∧ ¬Qx)) [∀-introduction (2-14)]

(c) ∀x∀y((¬Px ∨ ¬Qx) → ¬(Px ∧ Qx))

∀x∀y((¬Px ∨ ¬Qx) → ¬(Px ∧ Qx)) [Given]
Let a be an arbitrary element. [Assumption for universal introduction]
Let b be an arbitrary element. [Assumption for universal introduction]
(¬Pa ∨ ¬Qa) → ¬(Pa ∧ Qa) [Universal instantiation using a and b]
¬Pa ∨ ¬Qa [Assumption for →-elimination]
¬(Pa ∧ Qa) [Modus Ponens (4, 5)]
¬Pa [Assumption for ¬-elimination]
¬Qa [Assumption for ¬-elimination]
¬Pa ∨ ¬Qa [∨-introduction (7)]
¬(Pa ∧ Qa) [¬-elimination (6, 8)]
¬(Px ∧ Qx) [Universal instantiation using a (9, 10)]
¬(Px ∧ Qx) [¬-introduction (7-11)]
¬Px ∨ ¬Qx → ¬(Px ∧ Qx) [→-introduction (5-12)]
∀y((¬Px ∨ ¬Qx) → ¬(Px ∧ Qx)) [∀-introduction (3-13)]
∀x∀y((¬Px ∨ ¬Qx) → ¬(Px ∧ Qx)) [∀-introduction (2-14)]

(d) ∀x∀y((¬Px ∧ ¬Qx) → ¬(Px ∨ Qx))

∀x∀y((¬Px ∧ ¬Qx) → ¬(Px ∨ Qx)) [Given]
Let a be an arbitrary element. [Assumption for universal introduction]
Let b be an arbitrary element. [Assumption for universal introduction]
(¬Pa ∧ ¬Qa) → ¬(Pa ∨ Qa) [Universal instantiation using a and b]
(¬Pa ∧ ¬Qa) [Assumption for →-elimination]
¬(Pa ∨ Qa) [Modus Ponens (4, 5)]
¬Pa [Conjunction elimination (5)]
¬Qa [Conjunction elimination (5)]
¬(Pa ∨ Qa) [∧-elimination (7)]
¬Pa [¬-elimination (6, 8)]
¬Qa [¬-elimination (6, 8)]
¬Pa [∧-elimination (8)]
¬(Pa ∨ Qa) [¬-elimination (9)]
¬(Pa ∨ Qa) [→-introduction (5, 13)]
∀y((¬Pa ∧ ¬Qa) → ¬(Pa ∨ Qa)) [∀-introduction (3-14)]
∀x∀y((¬Px ∧ ¬Qx) → ¬(Px ∨ Qx)) [∀-introduction (2-15)]

We generate this asnwer using ChatGPT.
```
10. Compare and contrast the proofs provided for (a) in your answers to questions 8 and 9. Explain the different assumptions, strategies, etc. exhibited in tree proofs vs natural deduction proofs. 
 
 ```
 In the tree proof of "∀x∀y(¬(Px ∧ Qx) → (¬Px ∨ ¬Qx))," the strategy is to deny the conditional to get contradictions (indirect deduction strategy). The natural deduction proof for the statement uses the conditional deduction strategy.

 This was a tentative answer. To discuss more and improve.to ask to John too.

 We chacked Karl and Giacomo's answers.
 We report them here.
 Karl: "For (a), a Fitch-style natural deduction proof relies on deductive rules like disjunction elimination or double negation elimination (DNE) to a more substantive degree than a tree proof.
 While a Fitch-style natural deduction proof is a combinational application of different means of derivation, a tree proof is essentially an application of indirect derivation. That is, when we do a tree proof, we have to decompose the target (complex) formula into its subformulas, and then differently connect negations of those subformulas in order to form different paths. Once when all paths somehow involve a contradiction, then the opposite possibilities of the target formula are all shown to be implausible, and thus the target formula will be proved.
 Moreover, a Fitch-style natural deduction proof is to apply rules to the target formula and its logical consequents, while a tree proof does not apply the same rules but concentrates on finding possible logical contradictions among negated subformulas of the target formula."

 Giacomo: " The tree method starts by assuming the negation of the statement to prove. It then applies a set of rule of derivations in order to find closed branches which provide a countermodel to the negated statement and ultimately prove it wrong (thus proving the original statement). The natural deduction method instead breaks the statement into an assumption and a consequence and then applies rules which transform the original statement into the cnosequence. In alternative, it can negate the statement and reach a contradiction, thus proving the statement true. 8a) starts by negating the statement we want to prove, then gets rid of the quantifiers, then unwraps the negation of the implication, then applie rules to break down the disjunction in line 5 and then eliminates the double negation. We are left with either Qa or Pa being true. Buth both are in contradiction with the breaking down of line 4. Hence, the negated statement is contradictory and we have proved our initial goal. 9a) starts by assuming the antecedent inside the parenthesis. Then assumes the negation of the consequent. Then goes on to prove that this is contradictory, and prove the consequent starting from the antecedent. Even if there are proofs by contradiction inside of this strategy, it remains different from the tableau method because we started by assuming one of the elements and then proved that the other element followed from it. Using the tableau method, we rather tried to negate the whole statement and proved that it brings to a contradiction by exploring each possbility."
